Progress on alternate definition of decode_string_with_term.  Still missing invariant in the right conj and one other case.

src/Narcissus/Formats/WithTerm/String.v
@@ -10,6 +10,9 @@ Require Import
         Fiat.Narcissus.Formats.Delimiter
         Fiat.Narcissus.Formats.AsciiOpt.
 
+Require Import WordOpt.
+Require Import Bedrock.Word.
+
 Section String.
   Context {B : Type}.
   Context {cache : Cache}.
@@ -18,65 +21,206 @@ Section String.
   Context {monoidUnit : QueueMonoidOpt monoid bool}.
 
   Definition decode_string_with_term
-           (code: string)
-           (b : B) (cd : CacheDecode)
-    : option (string * B * CacheDecode) := 
-    (Fix well_founded_lt_b
+             (code: string)
+    :  B -> CacheDecode -> option (string * B * CacheDecode) := 
+      Fix well_founded_lt_b
            (fun _ => CacheDecode -> option (string * B * CacheDecode))
-      (fun b rec cd =>
-     `(term_code, b', cd') <- decode_string (String.length code) b cd;
-      (* (peekD (T := string) cd) *)
-      If String.eqb code term_code Then
-        Some (EmptyString, b', cd')
-      Else
-        (`(a, b1, e1) <- Decode_w_Measure_lt decode_ascii b cd ltac:(exact ascii_decode_lt);
-        (`(xs, b2, e2) <- rec _ (proj2_sig b1) e1;
-        Some (String a xs, b2, e2)))) b cd).
+         (fun b rec cd =>
+            match decode_string (String.length code) b cd with
+            | None => 
+              (`(a, b1, e1) <- Decode_w_Measure_lt decode_ascii b cd ltac:(exact ascii_decode_lt);
+              (`(xs, b2, e2) <- rec _ (proj2_sig b1) e1;
+              Some (String a xs, b2, e2)))
+            | Some((term_code, b', cd')) =>
+               If String.eqb code term_code Then
+                Some (EmptyString, b', cd')
+               Else
+                (`(a, b1, e1) <- Decode_w_Measure_lt decode_ascii b cd ltac:(exact ascii_decode_lt);
+                (`(xs, b2, e2) <- rec _ (proj2_sig b1) e1;
+                Some (String a xs, b2, e2)))
+            end).
 
+  Ltac unf H := 
+    repeat (
+    unfold DecodeBindOpt2 in H;
+    unfold BindOpt in H;
+    unfold If_Opt_Then_Else in H;
+    unfold DecodeBindOpt in H;
+    unfold Bind2 in H;
+    unfold BindOpt in H).
 
-  Lemma format_string_cons : 
-    forall (a : Ascii.ascii) (s : string) (s' : B) (env xenv : CacheFormat)
-           (close : string),
-      (format_string ++ format_string ◦ constant close) (String a s) env
-         ∋ (s', xenv) ->
-         exists s'' xenv' env' b,
-           (format_string ++ format_string ◦ constant close) s env' ∋ (s'', xenv') /\
-           mappend b s'' = s'.
+  Ltac unfg := 
+    repeat (unfold DecodeBindOpt2;
+    unfold BindOpt;
+    unfold If_Opt_Then_Else;
+    unfold DecodeBindOpt;
+    unfold Bind2;
+    unfold BindOpt).
+
+      
+  Lemma format_string_env_eq : forall s env env' b,
+      (format_string s env) ∋ (b, env') ->
+      env' = fold_left (fun acc elt =>
+                   (addE acc 8)) (list_ascii_of_string s) env.
+  Proof.
+    induction s; intros; auto.
+    {
+      simpl in H.
+      computes_to_inv.
+      inversion H; subst; auto.
+    }
+    {
+      simpl in H.
+    repeat match goal with
+                 | H : ComposeOpt.compose _ _ _ _ ∋ _ |- _ =>
+                   apply Bind_inv in H;
+                     destruct_ex;
+                     split_and
+                 | H : Bind2 _ _ ∋ _ |- _ =>
+                   apply Bind_inv in H;
+                     destruct_ex;
+                     split_and
+                 end.
+      computes_to_inv.
+      inversion H2.
+      subst.
+      clear H2.
+      unfold format_ascii in H0.
+      unfold WordOpt.format_word  in H0.    
+      computes_to_inv.
+      destruct x.
+      inversion H0; subst; auto.
+      clear H0.
+      simpl in H1.
+      destruct x0.
+      apply IHs in H1.
+      simpl.
+      subst; auto.
+    }
+  Qed.
+
+  Lemma fold_add_eq : forall B A (l : list B) env n (add : A -> nat -> A), 
+      (fold_left (fun acc : A => constant add acc n) l (add env n))
+      = add (fold_left (fun acc : A => constant add acc n) l env) n.
+  Proof.
+    induction l; simpl; auto; try auto using IHl.
+  Qed.
+
+  Lemma decode_string_env_eq : forall n s env cd env' (b : B),
+      decode_string n cd env = Some (s, b, env') ->
+      env' = fold_left (fun acc elt =>
+                   (addD acc 8)) (repeat 0 n) env.
+  Proof.
+    induction n; intros; auto.
+    {
+      simpl in H.
+      inversion H; subst; auto.
+    }
+    {
+      simpl in H.
+      unf H.
+      simpl.
+      destruct (decode_ascii cd env) eqn:Ha; try discriminate.
+      destruct p,p.
+      destruct (decode_string n b0 c) eqn:Hs; try discriminate.
+      destruct p,p.
+      inversion H; subst.
+      apply IHn in Hs.
+      assert (c = addD env 8); subst; auto.
+      {
+        clear -Ha.
+        unfold decode_ascii in Ha.
+        unfold decode_word in Ha.
+        destruct (decode_word' 8 cd); try discriminate.
+        simpl in Ha.
+        destruct p.
+        inversion Ha; auto.
+      }
+    }
+  Qed.
+
+  Lemma decode_word_invar : forall b b' env0 env n (w : word n) env', 
+      decode_word b env = Some (w, b', env0) ->
+      exists env0', 
+        decode_word b env' = Some(w, b', env0').
   Proof.
     intros.
-    apply Bind_inv in H;
-      destruct_ex;
-      split_and.
-    repeat match goal with
-        | H : ComposeOpt.compose _ _ _ _ ∋ _ |- _ =>
-          apply Bind_inv in H;
-            destruct_ex;
-            split_and
-        | H : Bind2 _ _ ∋ _ |- _ =>
-          apply Bind_inv in H;
-            destruct_ex;
-            split_and
-        end.
-        apply Return_inv in H2,H4.
-        inversion H4; subst.
-        clear H.
-        simpl in H2.
-        inversion H2.
-        subst.
-        clear H2.
-        exists (mappend (fst x2) (fst x0)).
-        exists (snd x0).
-        exists (snd x1).
-        eexists (fst x1).
-        split; eauto.
-        econstructor.
-        split; red; simpl; eauto.
-        exact H3.
-        simpl in *.
-        apply unfold_computes.
-        eapply BindComputes; eauto.
-        rewrite mappend_assoc.
-        auto.
+    unfold decode_word in *.
+    unf H.
+    unfg .
+    destruct (decode_word' n b) eqn:Hw.
+    inversion H.
+    subst; eauto.
+    discriminate.
+  Qed.
+
+  Lemma decode_ascii_env : forall b b' env0 env a env', 
+      decode_ascii b env = Some (a, b', env0) ->
+      exists env0', 
+        decode_ascii b env' = Some(a, b', env0').
+  Proof.
+    unfold decode_ascii.
+    intros.
+    unf H.
+    destruct (decode_word b env) eqn:H2; try discriminate.
+    destruct p,p.
+    eapply decode_word_invar in H2.
+    destruct H2 as [env0' H2]; rewrite H2.
+    simpl.
+    inversion H; subst; eauto.
+  Qed.
+
+  Definition head_option (s : string) :=
+    match s with
+    | EmptyString => None
+    | String a s' => Some a
+    end.
+
+  Lemma decode_string_ascii : forall n b ext env env0' s b' env', 
+      n <> 0 -> 
+      decode_string n (mappend b ext) env =
+      Some (s, b', env0') ->
+      exists b'' env'', 
+        decode_ascii (mappend b ext) env' =
+        option_map (fun a => (a, b'', env'' )) (head_option s).
+  Proof.
+    unfold option_map.
+    destruct n; 
+      intros; [
+        contradiction| ].
+    destruct n.
+    {
+      simpl in *.
+      unf H0.
+      destruct decode_ascii eqn:Ha in H0.
+      destruct p,p.
+      simpl in *.
+      eapply decode_ascii_env in Ha.
+      destruct Ha.
+      rewrite H1.
+      inversion H0; subst.
+      simpl.
+      eauto.
+      discriminate.
+    }
+    {
+      simpl in H0.
+      unf H0.
+      destruct decode_ascii eqn:Ha in H0; try discriminate.
+      destruct p,p.
+      eapply decode_ascii_env in Ha; try discriminate.
+      destruct_ex.
+      rewrite H1.
+      destruct decode_ascii eqn:Ha' in H0; try discriminate.
+      destruct p,p.
+      destruct decode_string eqn:Hs in H0; try discriminate.
+      destruct p,p.
+      simpl in *.
+      inversion H0.
+      subst.
+      simpl in *.
+      eauto.
+    }
   Qed.
 
   Theorem string_decode_with_term_correct
@@ -86,8 +230,8 @@ Section String.
                         (fun P0 : CacheDecode -> Prop =>
                           forall (b : nat) (cd : CacheDecode), P0 cd -> P0 (addD cd b))) :
     CorrectDecoder monoid
-                   (fun s => forall s1 s2, s <> s1 ++ close ++ s2)%string
-                   (fun s => forall s1 s2, s <> s1 ++ close ++ s2)%string
+                   (fun s => (forall s1 s2, s <> s1 ++ close ++ s2))%string
+                   (fun s => (forall s1 s2, s <> s1 ++ close ++ s2))%string
                    eq
                    (format_with_term format_string close)
                    (decode_string_with_term close)
@@ -98,153 +242,437 @@ Section String.
     { intros env env' xenv s s' ext ? Eeq Ppred Penc.
       generalize dependent env.
       revert env' xenv s' env_OK.
+      (* destruct Ppred as [Ppred Pclose]. *)
       induction s.
-      { unfold id in *; intros.
-        unfold format_with_term in Penc.
-        unfold "++" in Penc.
-        simpl in Penc.
-        unfold Bind2 in Penc.
-        apply Bind_inv in Penc.
-        destruct_ex.
-        split_and.
-        apply Return_inv in H0.
-        rewrite <- H0 in H1.
-        simpl in H1.
-        apply Bind_inv in H1.
-        destruct H1.
-        destruct H.
-        rewrite mempty_left in H1.
-        apply Return_inv in H1.
-        inversion H1; subst.
-        clear H1.
+      { unfold id in *; intros; unfold format_with_term in Penc;
+        unfold "++" in Penc; simpl in Penc;
+        unfold Bind2 in Penc; apply Bind_inv in Penc.
+        clear Ppred.
+        destruct_ex; split_and.
+        apply Return_inv in H0; rewrite <- H0 in H1; simpl in H1.
+        apply Bind_inv in H1; destruct H1; destruct H.
+        rewrite mempty_left in H1; apply Return_inv in H1.
+        inversion H1; subst; clear H1.
         pose proof H as Hsave.
         unfold decode_string_with_term.
         rewrite Init.Wf.Fix_eq.
-        destruct H.
-        split_and.
-        subst.
+        destruct H; split_and; subst.
         pose proof (String_decode_correct (P := P)).
         destruct H with (sz := String.length x); eauto.
         destruct x0.
         eapply H1 in H0; eauto.
         clear H H1 H2.
-        destruct_ex; split_and.
-        subst.
-        simpl.
-        rewrite H0.
-        simpl.
-        replace (x0 =? x0)%string with true by (auto using eqb_refl).
-        simpl.
+        destruct_ex; split_and; subst; simpl.
+        rewrite H0; simpl.
+        replace (x0 =? x0)%string with true by (auto using eqb_refl); simpl.
         exists ""%string, x1.
         {
-          intuition; auto.
-          unfold format_with_term.
-          econstructor; eauto.
+          intuition; auto; unfold format_with_term; econstructor; eauto.
           split.
-          unfold Ensembles.In.
-          simpl.
-          apply unfold_computes.
-          eapply ReturnComputes.
-          simpl.
-          red.
-          unfold Bind2.
-          apply unfold_computes.
-          eapply BindComputes; eauto.
-          rewrite mempty_left.
-          auto.
+          unfold Ensembles.In; simpl; apply unfold_computes; eapply ReturnComputes.
+          simpl; red; unfold Bind2. apply unfold_computes.
+          eapply BindComputes; eauto; rewrite mempty_left; auto.
         }
         {
-          intros.
-          repeat (apply functional_extensionality; intros; f_equal).
-          subst; auto.
-          unfold DecodeBindOpt2.
-          unfold BindOpt.
-          unfold If_Opt_Then_Else.
-          destruct Decode_w_Measure_lt; auto.
-          do 2 destruct p; rewrite H0; auto.
+          intros; 
+          repeat (apply functional_extensionality; intros; f_equal); unfg;
+          destruct Decode_w_Measure_lt; auto;
+          destruct_conjs;
+          match goal with| H : context[_ _ _ = _ _ _] |- _ => rewrite H end; auto.
         }
       }
       {
         intros.
-        unfold format_with_term in Penc;
-          unfold decode_string_with_term.
-        pose proof Penc as PencInd.
-        apply format_string_cons in PencInd.
-        destruct PencInd.
-        destruct_ex; split_and.
-        subst.
-        rename H0 into IHPenc.
-        simpl in *.
-        assert (IHpred : forall s1 s2 : string, s <> (s1 ++ close ++ s2)%string).
+        (* pose proof Penc as PencHold. *)
+        unfold format_with_term in Penc.
+        unfold "++" in Penc.
+        unfold ComposeOpt.compose in Penc.
+        (* exists (String a s). *)
+        unfold decode_string_with_term.
+        rewrite Init.Wf.Fix_eq.
+        (* assert (Deq : *)
+        (*     (`(a0, b1, e1) <- Decode_w_Measure_lt decode_ascii  *)
+        (*                       (mappend s' ext) env' ascii_decode_lt; *)
+        (*    `(xs, b2, e2) <- Fix well_founded_lt_b *)
+        (*                       (constant (CacheDecode -> *)
+        (*                                  option (string * B * CacheDecode))) *)
+        (*                       (fun (b : B) *)
+        (*                          (rec : forall y : B, *)
+        (*                                 lt_B y b -> *)
+        (*                                 CacheDecode -> *)
+        (*                                 option (string * B * CacheDecode)) *)
+        (*                          (cd : CacheDecode) => *)
+        (*                        `(term_code0, b'0, cd'0) <-  *)
+        (*                        decode_string (String.length close) b cd; *)
+        (*                        If (close =? term_code0)%string *)
+        (*                        Then Some (""%string, b'0, cd'0) *)
+        (*                        Else (`(a1, b0, e0) <- Decode_w_Measure_lt decode_ascii *)
+        (*                                                 b cd ascii_decode_lt; *)
+        (*                              `(xs, b2, e2) <- rec (` b0) (proj2_sig b0) e0; *)
+        (*                              Some (String a1 xs, b2, e2))) *)
+        (*                       (` b1) e1; *)
+        (*                        Some (String a0 xs, b2, e2)) *)
+        (*     =  *)
+        (*    (`(a0, b1, e1) <- Decode_w_Measure_lt decode_ascii  *)
+        (*                                          (mappend s' ext) env' ascii_decode_lt; *)
+        (*     `(xs, b2, e2) <- decode_string_with_term close (` b1) e1; *)
+        (*    Some (String a0 xs, b2, e2)) *)
+        (*   ) by auto. *)
+        assert (Deq :
+            (`(a0, b1, e1) <- Decode_w_Measure_lt decode_ascii 
+                              (mappend s' ext) env' ascii_decode_lt;
+           `(xs, b2, e2) <- Fix well_founded_lt_b
+                              (constant (CacheDecode ->
+                                         option (string * B * CacheDecode)))
+                              (fun (b : B)
+                                 (rec : forall y : B,
+                                        lt_B y b ->
+                                        CacheDecode ->
+                                        option (string * B * CacheDecode))
+                                 (cd : CacheDecode) =>
+                               match decode_string (String.length close) b cd with
+                            | Some (term_code, b', cd') =>
+                                If (close =? term_code)%string
+                                Then Some (""%string, b', cd')
+                                Else (`(a1, b0, e0) <- Decode_w_Measure_lt decode_ascii
+                                                         b cd ascii_decode_lt;
+                                      `(xs, b2, e2) <- rec (` b0) (proj2_sig b0) e0;
+                                      Some (String a1 xs, b2, e2))
+                            | None =>
+                                `(a1, b0, e0) <- Decode_w_Measure_lt decode_ascii b cd
+                                                   ascii_decode_lt;
+                                `(xs, b2, e2) <- rec (` b0) (proj2_sig b0) e0;
+                                Some (String a1 xs, b2, e2)
+                            end)
+                              (` b1) e1;
+                               Some (String a0 xs, b2, e2))
+            = 
+           (`(a0, b1, e1) <- Decode_w_Measure_lt decode_ascii 
+                                                 (mappend s' ext) env' ascii_decode_lt;
+            `(xs, b2, e2) <- decode_string_with_term close (` b1) e1;
+           Some (String a0 xs, b2, e2))
+          ) by auto.
+        rewrite Deq.
+        clear Deq.
+        assert (IHpred : (forall s1 s2 : string, s <> s1 ++ close ++ s2)%string).
         {
           clear -Ppred.
           intros.
           specialize (Ppred (String a s1) s2).
           intros Hnot.
-          subst.
-          simpl in *.
-          auto.
+          subst; eauto.
         }
         specialize (IHs IHpred).
         clear IHpred.
-        eapply IHs in IHPenc; eauto.
-        destruct_ex; split_and.
-        (* subst. *)
-        {
-          unfold "++" in Penc.
-          apply Bind_inv in Penc;
-            destruct_ex;
+        unfold Bind2 in Penc.
+        computes_to_inv.
+        destruct_conjs.
+        simpl fst in *.
+        simpl snd in *.
+        inversion Penc''.
+        subst.
+        clear Penc''.
+        simpl in Penc.
+        unf Penc.
+        computes_to_inv.
+        destruct_conjs.
+        simpl in *.
+        apply EquivFormat_Projection_Format in Penc'.
+        (* eapply String_decode_correct with (sz := String.length close) in Penc'. *)
+        (* destruct_ex. *)
+        (* split_and. *)
+        (* rewrite <- H in *. *)
+        (* clear H. *)
+        destruct (decode_string (String.length close)
+                                (mappend (mappend b0 b) ext) env') eqn:Hs.
+        2:{
+            simpl.
+            (* clear H0. *)
+            clear Hs.
+            eapply Ascii_decode_correct in Penc; eauto.
+            set (forall s1 s2, String a s <> (s1 ++ close ++ s2)%string /\ close <> ""%string) as f in Ppred.
+            destruct_ex.
             split_and.
-          unfold format_with_term in IHs.
-          repeat match goal with
-                 | H : ComposeOpt.compose _ _ _ _ ∋ _ |- _ =>
-                   apply Bind_inv in H;
-                     destruct_ex;
-                     split_and
-                 | H : Bind2 _ _ ∋ _ |- _ =>
-                   apply Bind_inv in H;
-                     destruct_ex;
-                     split_and
-                 end.
-          apply Return_inv in H7,H9.
-          (* inversion H8; subst. *)
-          (* clear H. *)
-          (* simpl in H7. *)
-          simpl in *.
-          unfold format_with_term in H1.
-          pose proof (String_decode_correct (P := P)) as Hs.
-          destruct Hs with (sz := String.length close); eauto.
-          clear H10 Hs.
-          destruct x6.
-          simpl in *.
-          inversion H6; subst.
-          destruct H10.
-          subst.
-          simpl in *.
-          inversion H7; subst.
-          simpl in *.
-          (* exists (String a x3). *)
-          rewrite Init.Wf.Fix_eq.
-          eexists; eauto.
-          eexists; eauto.
+            pose proof H0 as Hhold.
+            eapply Decode_w_Measure_lt_eq in H0.
+            destruct_ex.
+            inversion Penc'0'.
+            rewrite <- mappend_assoc.
+            rewrite <- mappend_assoc.
+            rewrite H0.
+            simpl.
+            assert (format_with_term format_string close s c1 ∋
+                                     (mappend b1 b, xenv)).
+            {
+              subst.
+              unfold format_with_term.
+              unfold "++".
+              unfold ComposeOpt.compose.
+              computes_to_econstructor; eauto.
+              computes_to_econstructor; eauto.
+              apply EquivFormat_Projection_Format; simpl; eauto.
+              simpl.
+              eauto.
+            }
+            {
+              eapply IHs in H3; eauto.
+              destruct_ex.
+              split_and.
+              rewrite mappend_assoc.
+              rewrite H7; eauto.
+              simpl; eauto.
+              eexists.
+              eexists.
+              split; eauto.
+              split; subst; eauto.
+              split; eauto.
+              computes_to_econstructor; eauto.              
+              simpl.
+              computes_to_econstructor; eauto.
+              computes_to_econstructor; eauto.
+              simpl.
+              computes_to_econstructor; eauto.
+              epose proof (EquivFormat_Projection_Format (format_string)).
+              red in H.
+              red in H.
+              specialize (H (constant close) (String x x2) c0).
+              destruct H.
+              red in H.
+              apply H.
+              eauto.
+              eauto.
+            }
+        }
+        {
+          destruct p,p.
+          simpl.
+          destruct String.eqb eqn:?.
+          simpl.
           {
-          
-            apply EquivFormat_Projection_Format in H6.
-            eapply (@H3 _ _ _ _ _ ext) in H6; eauto.
-            clear H3.
+            admit.
+          }
+          {
+            simpl.
+            (* clear H0. *)
+            clear Hs.
+            eapply Ascii_decode_correct in Penc; eauto.
+            destruct_ex.
+            split_and.
+            pose proof H0 as Hhold.
+            eapply Decode_w_Measure_lt_eq in H0.
+            destruct_ex.
+            inversion Penc'0'.
+            rewrite <- mappend_assoc.
+            rewrite <- mappend_assoc.
+            rewrite H0.
+            simpl.
+            assert (format_with_term format_string close s c1 ∋
+                                     (mappend b1 b, xenv)).
+            {
+              subst.
+              unfold format_with_term.
+              unfold "++".
+              unfold ComposeOpt.compose.
+              computes_to_econstructor; eauto.
+              computes_to_econstructor; eauto.
+              apply EquivFormat_Projection_Format; simpl; eauto.
+              simpl.
+              eauto.
+            }
+            {
+              eapply IHs in H3; eauto.
+              destruct_ex.
+              split_and.
+              rewrite mappend_assoc.
+              rewrite H7; eauto.
+              simpl; eauto.
+              eexists.
+              eexists.
+              split; eauto.
+              split; subst; eauto.
+              split; eauto.
+              computes_to_econstructor; eauto.              
+              simpl.
+              computes_to_econstructor; eauto.
+              computes_to_econstructor; eauto.
+              simpl.
+              computes_to_econstructor; eauto.
+              epose proof (EquivFormat_Projection_Format (format_string)).
+              red in H.
+              red in H.
+              specialize (H (constant close) (String x x2) c0).
+              destruct H.
+              red in H.
+              apply H.
+              eauto.
+              eauto.
+            }
+          }
+        }
+        {
+          intros; 
+          repeat (apply functional_extensionality; intros; f_equal); unfg;
+          destruct Decode_w_Measure_lt; auto;
+          destruct_conjs;
+          match goal with| H : context[_ _ _ = _ _ _] |- _ => rewrite H end; auto.
+        }
+      }
+    }
+    { unfold decode_string_with_term, format_with_term;
+        intros env env' xenv' data bin;
+        revert env env' xenv' data.
+      eapply (@well_founded_induction _ _ well_founded_lt_b) with
+      (a := bin); intros.
+      rewrite Coq.Init.Wf.Fix_eq in H2; auto; simpl.
+      destruct (decode_string (String.length close) x env') eqn:Hc.
+      {
+        destruct p,p.
+        destruct (close =? s)%string eqn:Heqc.
+        {
+          simpl in H2.
+          inversion H2; subst.
+          split; eauto.
+          {
+            apply decode_string_env_eq in Hc.
+            subst; eauto.
+            clear - H1 cache_inv.
+            induction (String.length close); auto.
+            simpl.
+            rewrite fold_add_eq; auto.
+          }
+          pose proof Hc as Hclose.
+          eapply @String_decode_correct in Hc; eauto.
+          destruct Hc.
+          destruct_ex.
+          eexists.
+          eexists.
+          split; eauto.
+          clear H2.
+          computes_to_econstructor; eauto.
+          {
+            computes_to_econstructor; eauto.
+          }
+          {
+            computes_to_econstructor; eauto.
+            epose proof (EquivFormat_Projection_Format (format_string)).
+            red in H2.
+            red in H2.
+            specialize (H2 (constant close) ""%string env).
+            destruct H2.
+            red in H2.
+            simpl.
+            apply H2.
+            clear H2 H3.
             destruct_ex; split_and.
-            clear IHs.
-            inversion H7; subst.
-            unfold decode_string_with_term in H0.
-            (* Really close here just need to know that decode_string 
-               returns some on bigger args if it did for smaller ones 
-               and that the string it results in is not the same 
-               and that it is not equal to close using H6
-             *)
-            (* Then we can hopefully use the decode_ascii in scope and 
-               the result of our induction hypothesis to prove the rec bind 
-               is some of something 
-             *)
-            (* Haven't thought about the other conjuncts. *)
-  Admitted.
-End String.
+            clear H6 H8.
+            apply eqb_eq in Heqc.
+            Unshelve.
+            2:{
+              exact (x0, x1).
+            }
+            rewrite Heqc.
+            exact H2.
+          }
+          {
+            intuition; subst; simpl; auto.
+            rewrite mempty_left; auto.
+            admit.
+          }
+        }
+        {
+          simpl in H2.
+          apply DecodeBindOpt2_inv in H2;
+            destruct H2 as [? [? [? [? ?] ] ] ]; injections; subst.
+          destruct (decode_ascii x env') as [ [ [? ?] ?] | ] eqn: ? .
+          - destruct (Decode_w_Measure_lt_eq _ _ _ ascii_decode_lt Heqo).
+            rewrite H4 in H2; injections.
+            eapply (proj2 (Ascii_decode_correct cache_inv)) in Heqo; eauto;
+            destruct Heqo as [? [? ?] ]; destruct_ex.
+            symmetry in H3; apply DecodeBindOpt2_inv in H3;
+            destruct H3 as [? [? [? [? ?] ] ] ]; injections; subst.
+            eapply H in H3; intuition.
+            destruct_ex; intuition; subst; eauto.
+            unfold "++" in H9.
+            unfold ComposeOpt.compose in H9.
+            unfold Bind2 in H9.
+            computes_to_inv.
+            eexists _, _; intuition.
+            {
+              computes_to_econstructor; eauto.
+              -
+                simpl.
+                computes_to_econstructor; eauto.
+                computes_to_econstructor; eauto.
+              -
+                computes_to_econstructor; eauto.
+            }
+            {
+              destruct_conjs; simpl in *; subst.
+              inversion H9''; subst.
+              do 2 rewrite mappend_assoc; auto.
+            }
+            {
+              admit.
+            }
+            {
+              destruct_conjs; simpl in *;
+              inversion H9''; subst; auto.
+            }
+            {
+              auto.
+            }
+          - eapply Decode_w_Measure_lt_eq' in Heqo; rewrite Heqo in H2;
+              discriminate.
+        }
+      }
+      {
+        apply DecodeBindOpt2_inv in H2;
+            destruct H2 as [? [? [? [? ?] ] ] ]; injections; subst.
+        destruct (decode_ascii x env') as [ [ [? ?] ?] | ] eqn: ? .
+        - destruct (Decode_w_Measure_lt_eq _ _ _ ascii_decode_lt Heqo).
+            rewrite H4 in H2; injections.
+            eapply (proj2 (Ascii_decode_correct cache_inv)) in Heqo; eauto;
+            destruct Heqo as [? [? ?] ]; destruct_ex.
+            symmetry in H3; apply DecodeBindOpt2_inv in H3;
+            destruct H3 as [? [? [? [? ?] ] ] ]; injections; subst.
+            eapply H in H3; intuition.
+            destruct_ex; intuition; subst; eauto.
+            unfold "++" in H9.
+            unfold ComposeOpt.compose in H9.
+            unfold Bind2 in H9.
+            computes_to_inv.
+            eexists _, _; intuition.
+            {
+              computes_to_econstructor; eauto.
+              -
+                simpl.
+                computes_to_econstructor; eauto.
+                computes_to_econstructor; eauto.
+              -
+                computes_to_econstructor; eauto.
+            }
+            {
+              destruct_conjs; simpl in *; subst.
+              inversion H9''; subst.
+              do 2 rewrite mappend_assoc; auto.
+            }
+            {
+              admit.
+            }
+            {
+              destruct_conjs; simpl in *; subst;
+              inversion H9''; subst; auto.
+            }
+            {
+              auto.
+            }
+        - eapply Decode_w_Measure_lt_eq' in Heqo; rewrite Heqo in H2;
+            discriminate.
+      }
+      intros; 
+        repeat (apply functional_extensionality; intros; f_equal); unfg;
+        destruct Decode_w_Measure_lt; auto;
+        destruct_conjs;
+        match goal with| H : context[_ _ _ = _ _ _] |- _ => rewrite H end; auto.
+    }
+    Admitted.
